Misc/MonadEquiv.v
@@ -26,5 +26,48 @@ Instance JoinToBind (M : Type -> Type) (inst : Join.Monad M) : Bind.Monad M :=
         (fmap f .> Join.join) ma
 }.
 Proof.
+(*  Focus 2. intros. Print Join.Monad. unfold compose.*)
   intros.
+  unfold compose.
+  Print Join.Monad.
+  assert (H := Join.join_law).
+  specialize (H A). unfold compose in H.
+  Print Applicative.
+  Print Functor.
+  Search Join.join.
+  Search Join.ret.
+  cut (fmap f (Join.ret a) = Join.ret (f a)).
+    intros ->.
+    Focus 2.
+
+Abort.
+
+Instance BindToComp (M : Type -> Type) (inst : Bind.Monad M)
+  : Comp.Monad M :=
+{
+    is_functor := @Bind.is_functor M inst;
+    ret := @Bind.ret M inst;
+    compM := fun (A B C : Type) (f : A -> M B) (g : B -> M C) =>
+        fun a : A => Bind.bind (f a) g
+}.
+Proof.
+  all: intros; extensionality x.
+    rewrite Bind.assoc. reflexivity.
+    apply Bind.id_left.
+    apply Bind.id_right.
+Defined.
+
+Instance BindToJoin (M : Type -> Type) (inst : Bind.Monad M)
+  : Join.Monad M :=
+{
+    is_functor := @Bind.is_functor M inst;
+    ret := @Bind.ret M inst;
+    join := fun (A : Type) (x : M (M A)) =>
+        Bind.bind x id
+}.
+Proof.
+  intros. unfold compose. extensionality x.
+    rewrite Bind.assoc.
+  Focus 2. intros. Print Bind.Monad. unfold compose.
+    extensionality x. rewrite Bind.id_left.
 Abort.
